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Chapter 1 - Introduction

Exercise 1

double (double 2)
= { applying the inner double }

double (2 + 2)
= { applying double }

(2 + 2) + (2 + 2)
= { applying the first + }

4 + (2 + 2)
= { applying the second + }

4 + 4
= { applying + }

8

or

double (double 2)
= { applying the outer double }

(double 2) + (double 2)
= { applying the second double }

(double 2) + (2 + 2)
= { applying the second + }

(double 2) + 4
= { applying double }

(2 + 2) + 4
= { applying the first + }

4 + 4
= { applying + }

8

There are a number of other answers too.

Exercise 2

sum [x ]
= { applying sum }

x + sum [ ]
= { applying sum }

x + 0
= { applying + }

x

Exercise 3

(1)

product [ ] = 1
product (x : xs) = x ∗ product xs
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(2)

product [2, 3, 4]
= { applying product }

2 ∗ (product [3, 4])
= { applying product }

2 ∗ (3 ∗ product [4])
= { applying product }

2 ∗ (3 ∗ (4 ∗ product [ ]))
= { applying product }

2 ∗ (3 ∗ (4 ∗ 1))
= { applying ∗ }

24

Exercise 4

Replace the second equation by

qsort (x : xs) = qsort larger ++ [x ] ++ qsort smaller

That is, just swap the occurrences of smaller and larger .

Exercise 5

Duplicate elements are removed from the sorted list. For example:

qsort [2, 2, 3, 1, 1]
= { applying qsort }

qsort [1, 1] ++ [2] ++ qsort [3]
= { applying qsort }

(qsort [ ] ++ [1] ++ qsort [ ]) ++ [2] ++ (qsort [ ] ++ [3] ++ qsort [ ])
= { applying qsort }

([ ] ++ [1] ++ [ ]) ++ [2] ++ ([ ] ++ [3] ++ [ ])
= { applying ++ }

[1] ++ [2] ++ [3]
= { applying ++ }

[1, 2, 3]
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Chapter 2 - First steps

Exercise 1

(2 ↑ 3) ∗ 4

(2 ∗ 3) + (4 ∗ 5)

2 + (3 ∗ (4 ↑ 5))

Exercise 2

No solution required.

Exercise 3

n = a ‘div ‘ length xs
where

a = 10
xs = [1, 2, 3, 4, 5]

Exercise 4

last xs = head (reverse xs)

or

last xs = xs !! (length xs − 1)

Exercise 5

init xs = take (length xs − 1) xs

or

init xs = reverse (tail (reverse xs))
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Chapter 3 - Types and classes

Exercise 1

[Char ]

(Char ,Char ,Char )

[(Bool ,Char )]

([Bool ], [Char ])

[[a ]→ [a ] ]

Exercise 2

[a ]→ a

(a, b)→ (b, a)

a → b → (a, b)

Num a ⇒ a → a

Eq a ⇒ [a ]→ Bool

(a → a)→ a → a

Exercise 3

No solution required.

Exercise 4

In general, checking if two functions are equal requires enumerating all possible ar-
gument values, and checking if the functions give the same result for each of these
values. For functions with a very large (or infinite) number of argument values, such
as values of type Int or Integer , this is not feasible. However, for small numbers of
argument values, such as values of type of type Bool , it is feasible.
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Chapter 4 - Defining functions

Exercise 1

halve xs = splitAt (length xs ‘div ‘ 2) xs

or

halve xs = (take n xs , drop n xs)
where

n = length xs ‘div ‘ 2

Exercise 2

(a)

safetail xs = if null xs then [ ] else tail xs

(b)

safetail xs | null xs = [ ]
| otherwise = tail xs

(c)

safetail [ ] = [ ]
safetail xs = tail xs

or

safetail [ ] = [ ]
safetail ( : xs) = xs

Exercise 3

(1)

False ∨ False = False
False ∨ True = True
True ∨ False = True
True ∨ True = True

(2)

False ∨ False = False
∨ = True

(3)

False ∨ b = b
True ∨ = True

(4)

b ∨ c | b == c = b
| otherwise = True
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Exercise 4

a ∧ b = if a then
if b then True else False

else
False

Exercise 5

a ∧ b = if a then b else False

Exercise 6

mult = λx → (λy → (λz → x ∗ y ∗ z ))
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Chapter 5 - List comprehensions

Exercise 1

sum [x ↑ 2 | x ← [1 . . 100]]

Exercise 2

replicate n x = [x | ← [1 . .n ] ]

Exercise 3

pyths n = [(x , y, z ) | x ← [1 . .n ],
y ← [1 . .n ],
z ← [1 . .n ],
x ↑ 2 + y ↑ 2 == z ↑ 2]

Exercise 4

perfects n = [x | x ← [1 . .n ], sum (init (factors x )) == x ]

Exercise 5

concat [ [(x , y) | y ← [4, 5, 6]] | x ← [1, 2, 3]]

Exercise 6

positions x xs = find x (zip xs [0 . .n ])
where n = length xs − 1

Exercise 7

scalarproduct xs ys = sum [x ∗ y | (x , y)← zip xs ys ]

Exercise 8

shift :: Int → Char → Char
shift n c | isLower c = int2low ((low2int c + n) ‘mod ‘ 26)

| isUpper c = int2upp ((upp2int c + n) ‘mod ‘ 26)
| otherwise = c

freqs :: String → [Float ]
freqs xs = [percent (count x xs ′) n | x ← [’a’ . . ’z’] ]

where
xs ′ = map toLower xs
n = letters xs

low2int :: Char → Int
low2int c = ord c − ord ’a’
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int2low :: Int → Char
int2low n = chr (ord ’a’+ n)

upp2int :: Char → Int
upp2int c = ord c − ord ’A’

int2upp :: Int → Char
int2upp n = chr (ord ’A’+ n)

letters :: String → Int
letters xs = length [x | x ← xs, isAlpha x ]
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Chapter 6 - Recursive functions

Exercise 1

(1)

m ↑ 0 = 1
m ↑ (n + 1) = m ∗m ↑ n

(2)

2 ↑ 3
= { applying ↑ }

2 ∗ (2 ↑ 2)
= { applying ↑ }

2 ∗ (2 ∗ (2 ↑ 1))
= { applying ↑ }

2 ∗ (2 ∗ (2 ∗ (2 ↑ 0)))
= { applying ↑ }

2 ∗ (2 ∗ (2 ∗ 1))
= { applying ∗ }

8

Exercise 2

(1)

length [1, 2, 3]
= { applying length }

1 + length [2, 3]
= { applying length }

1 + (1 + length [3])
= { applying length }

1 + (1 + (1 + length [ ]))
= { applying length }

1 + (1 + (1 + 0))
= { applying + }

3

(2)

drop 3 [1, 2, 3, 4, 5]
= { applying drop }

drop 2 [2, 3, 4, 5]
= { applying drop }

drop 1 [3, 4, 5]
= { applying drop }

drop 0 [4, 5]
= { applying drop }

[4, 5]
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(3)

init [1, 2, 3]
= { applying init }

1 : init [2, 3]
= { applying init }

1 : 2 : init [3]
= { applying init }

1 : 2 : [ ]
= { list notation }

[1, 2]

Exercise 3

and [ ] = True
and (b : bs) = b ∧ and bs

concat [ ] = [ ]
concat (xs : xss) = xs ++ concat xss

replicate 0 = [ ]
replicate (n + 1) x = x : replicate n x

(x : ) !! 0 = x
( : xs) !! (n + 1) = xs !! n

elem x [ ] = False
elem x (y : ys) | x == y = True

| otherwise = elem x ys

Exercise 4

merge [ ] ys = ys
merge xs [ ] = xs
merge (x : xs) (y : ys) = if x ≤ y then

x : merge xs (y : ys)
else

y : merge (x : xs) ys

Exercise 5

halve xs = splitAt (length xs ‘div ‘ 2) xs

msort [ ] = [ ]
msort [x ] = [x ]
msort xs = merge (msort ys) (msort zs)

where (ys , zs) = halve xs
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Exercise 6.1

Step 1: define the type

sum :: [Int ]→ Int

Step 2: enumerate the cases

sum [ ] =
sum (x : xs) =

Step 3: define the simple cases

sum [ ] = 0
sum (x : xs) =

Step 4: define the other cases

sum [ ] = 0
sum (x : xs) = x + sum xs

Step 5: generalise and simplify

sum :: Num a ⇒ [a ]→ a
sum = foldr (+) 0

Exercise 6.2

Step 1: define the type

take :: Int → [a ]→ [a ]

Step 2: enumerate the cases

take 0 [ ] =
take 0 (x : xs) =
take (n + 1) [ ] =
take (n + 1) (x : xs) =

Step 3: define the simple cases

take 0 [ ] = [ ]
take 0 (x : xs) = [ ]
take (n + 1) [ ] = [ ]
take (n + 1) (x : xs) =

Step 4: define the other cases

take 0 [ ] = [ ]
take 0 (x : xs) = [ ]
take (n + 1) [ ] = [ ]
take (n + 1) (x : xs) = x : take n xs

Step 5: generalise and simplify

take :: Int → [a ]→ [a ]
take 0 = [ ]
take (n + 1) [ ] = [ ]
take (n + 1) (x : xs) = x : take n xs
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Exercise 6.3

Step 1: define the type

last :: [a ]→ [a ]

Step 2: enumerate the cases

last (x : xs) =

Step 3: define the simple cases

last (x : xs) | null xs = x
| otherwise =

Step 4: define the other cases

last (x : xs) | null xs = x
| otherwise = last xs

Step 5: generalise and simplify

last :: [a ]→ [a ]
last [x ] = x
last ( : xs) = last xs
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Chapter 7 - Higher-order functions

Exercise 1

map f (filter p xs)

Exercise 2

all p = and ◦map p

any p = or ◦map p

takeWhile [ ] = [ ]
takeWhile p (x : xs)
| p x = x : takeWhile p xs
| otherwise = [ ]

dropWhile [ ] = [ ]
dropWhile p (x : xs)
| p x = dropWhile p xs
| otherwise = x : xs

Exercise 3

map f = foldr (λx xs → f x : xs) [ ]

filter p = foldr (λx xs → if p x then x : xs else xs) [ ]

Exercise 4

dec2nat = foldl (λx y → 10 ∗ x + y) 0

Exercise 5

The functions being composed do not all have the same types. For example:

sum :: [Int ]→ Int

map (↑2) :: [Int ]→ [Int ]

filter even :: [Int ]→ [Int ]

Exercise 6

curry :: ((a, b)→ c)→ (a → b → c)
curry f = λx y → f (x , y)

uncurry :: (a → b → c)→ ((a, b)→ c)
uncurry f = λ(x , y)→ f x y
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Exercise 7

chop8 = unfold null (take 8) (drop 8)

map f = unfold null (f ◦ head) tail

iterate f = unfold (const False) id f

Exercise 8

encode :: String → [Bit ]
encode = concat ◦map (addparity ◦make8 ◦ int2bin ◦ ord)

decode :: [Bit ]→ String
decode = map (chr ◦ bin2int ◦ checkparity) ◦ chop9

addparity :: [Bit ]→ [Bit ]
addparity bs = (parity bs) : bs

parity :: [Bit ]→ Bit
parity bs | odd (sum bs) = 1

| otherwise = 0

chop9 :: [Bit ]→ [ [Bit ] ]
chop9 [ ] = [ ]
chop9 bits = take 9 bits : chop9 (drop 9 bits)

checkparity :: [Bit ]→ [Bit ]
checkparity (b : bs)
| b == parity bs = bs
| otherwise = error "parity mismatch"

Exercise 9

No solution required.
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Chapter 8 - Functional parsers

Exercise 1

int = do char ’-’
n ← nat
return (−n)

+++nat

Exercise 2

comment = do string "--"
many (sat (
= ’\n’))
return ()

Exercise 3
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Exercise 4

(1)
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Exercise 5

Without left-factorising the grammar, the resulting parser would backtrack excessively
and have exponential time complexity in the size of the expression. For example, a
number would be parsed four times before being recognised as an expression.

Exercise 6

expr = do t ← term
do symbol "+"

e ← expr
return (t + e)

+++ do symbol "-"
e ← expr
return (t − e)

+++ return t

term = do f ← factor
do symbol "*"

t ← term
return (f ∗ t)

+++ do symbol "/"
t ← term
return (f ‘div ‘ t)

+++ return f

Exercise 7

(1)

factor ::= atom (↑ factor | epsilon)

atom ::= (expr) | nat

(2)

factor :: Parser Int
factor = do a ← atom

do symbol "^"
f ← factor
return (a ↑ f )

+++ return a

atom :: Parser Int
atom = do symbol "("

e ← expr
symbol ")"
return e

+++ natural
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Exercise 8

(a)

expr ::= expr − nat | nat

nat ::= 0 | 1 | 2 | · · ·
(b)

expr = do e ← expr
symbol "-"
n ← natural
return (e − n)

+++ natural

(c)

The parser loops forever without producing a result, because the first
operation it performs is to call itself recursively.

(d)

expr = do n ← natural
ns ← many (do symbol "-"

natural)
return (foldl (−) n ns)
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Chapter 9 - Interactive programs

Exercise 1

readLine = get ""

get xs = do x ← getChar
case x of

’\n’→ return xs
’\DEL’→ if null xs then

get xs
else

do putStr "\ESC[1D \ESC[1D"
get (init xs)

→ get (xs ++ [x ])

Exercise 2

No solution available.

Exercise 3

No solution available.

Exercise 4

No solution available.

Exercise 5

No solution available.

Exercise 6

type Board = [Int ]

initial :: Board
initial = [5, 4, 3, 2, 1]

finished :: Board → Bool
finished b = all (== 0) b

valid :: Board → Int → Int → Bool
valid b row num = b !! (row − 1) ≥ num

move :: Board → Int → Int → Board
move b row num = [if r == row then n − num else n

| (r ,n)← zip [1 . . 5] b ]
newline :: IO ()
newline = putChar ’\n’
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putBoard :: Board → IO ()
putBoard [a, b, c, d , e ] = do putRow 1 a

putRow 2 b
putRow 3 c
putRow 4 d
putRow 5 e

putRow :: Int → Int → IO ()
putRow row num = do putStr (show row)

putStr ": "
putStrLn (stars num)

stars :: Int → String
stars n = concat (replicate n "* ")

getDigit :: String → IO Int
getDigit prom = do putStr prom

x ← getChar
newline
if isDigit x then

return (ord x − ord ’0’)
else

do putStrLn "ERROR: Invalid digit"
getDigit prom

nim :: IO ()
nim = play initial 1

play :: Board → Int → IO ()
play board player = do newline

putBoard board
if finished board then

do newline
putStr "Player "
putStr (show (next player ))
putStrLn " wins!!"

else
do newline

putStr "Player "
putStrLn (show player )
r ← getDigit "Enter a row number: "
n ← getDigit "Stars to remove : "
if valid board r n then

play (move board r n) (next player )
else

do newline
putStrLn "ERROR: Invalid move"
play board player

next :: Int → Int
next 1 = 2
next 2 = 1

20



Chapter 10 - Declaring types and classes

Exercise 1

mult m Zero = Zero
mult m (Succ n) = add m (mult m n)

Exercise 2

occurs m (Leaf n) = m == n
occurs m (Node l n r) = case compare m n of

LT → occurs m l
EQ → True
GT → occurs m r

This version is more efficient because it only requires one comparison for each node,
whereas the previous version may require two comparisons.

Exercise 3

leaves (Leaf ) = 1
leaves (Node l r) = leaves l + leaves r

balanced (Leaf ) = True
balanced (Node l r) = abs (leaves l − leaves r) ≤ 1

∧ balanced l ∧ balanced r

Exercise 4

halve xs = splitAt (length xs ‘div ‘ 2) xs

balance [x ] = Leaf x
balance xs = Node (balance ys) (balance zs)

where (ys , zs) = halve xs

Exercise 5

data Prop = · · · | Or Prop Prop | Equiv Prop Prop

eval s (Or p q) = eval s p ∨ eval s q
eval s (Equiv p q) = eval s p == eval s q

vars (Or p q) = vars p ++ vars q
vars (Equiv p q) = vars p ++ vars q

Exercise 6

No solution available.
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Exercise 7

data Expr = Val Int | Add Expr Expr | Mult Expr Expr

type Cont = [Op ]

data Op = EVALA Expr | ADD Int | EVALM Expr | MUL Int

eval :: Expr → Cont → Int
eval (Val n) ops = exec ops n
eval (Add x y) ops = eval x (EVALA y : ops)
eval (Mult x y) ops = eval x (EVALM y : ops)

exec :: Cont → Int → Int
exec [ ] n = n
exec (EVALA y : ops) n = eval y (ADD n : ops)
exec (ADD n : ops) m = exec ops (n + m)
exec (EVALM y : ops) n = eval y (MUL n : ops)
exec (MUL n : ops) m = exec ops (n ∗m)

value :: Expr → Int
value e = eval e [ ]

Exercise 8

instance Monad Maybe where
return :: a → Maybe a
return x = Just x

(>>=) :: Maybe a → (a → Maybe b)→ Maybe b
Nothing >>= = Nothing
(Just x ) >>= f = f x

instance Monad [ ] where
return :: a → [a ]
return x = [x ]

(>>=) :: [a ]→ (a → [b ])→ [b ]
xs >>= f = concat (map f xs)
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Chapter 11 - The countdown problem

Exercise 1

choices xs = [zs | ys ← subs xs, zs ← perms ys ]

Exercise 2

removeone x [ ] = [ ]
removeone x (y : ys)
| x == y = ys
| otherwise = y : removeone x ys

isChoice [ ] = True
isChoice (x : xs) [ ] = False
isChoice (x : xs) ys = elem x ys ∧ isChoice xs (removeone x ys)

Exercise 3

It would lead to non-termination, because recursive calls to exprs would no longer be
guaranteed to reduce the length of the list.

Exercise 4

> length [e | ns ′ ← choices [1, 3, 7, 10, 25, 50], e ← exprs ns ]
33665406

> length [e | ns ′ ← choices [1, 3, 7, 10, 25, 50], e ← exprs ns, eval e 
= [ ]]
4672540

Exercise 5

Modifying the definition of valid by

valid Sub x y = True
valid Div x y = y 
= 0 ∧ x ‘mod ‘ y == 0

gives

> length [e | ns ′ ← choices [1, 3, 7, 10, 25, 50], e ← exprs ns ′, eval e 
= [ ]]
10839369

Exercise 6

No solution available.
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Chapter 12 - Lazy evaluation

Exercise 1

(1)

2 ∗ 3 is the only redex, and is both innermost and outermost.

(2)

1 + 2 and 2 + 3 are redexes, with 1 + 2 being innermost.

(3)

1 + 2, 2 + 3 and fst (1 + 2, 2 + 3) are redexes, with the first of these being
innermost and the last being outermost.

(4)

2 ∗ 3 and (λx → 1 + x ) (2 ∗ 3) are redexes, with the first being innermost
and the second being outermost.

Exercise 2

Outermost:

fst (1 + 2, 2 + 3)
= { applying fst }

1 + 2
= { applying + }

3

Innermost:

fst (1 + 2, 2 + 3)
= { applying the first + }

fst (3, 2 + 3)
= { applying + }

fst (3, 5)
= { applying fst }

3

Outermost evaluation is preferable because it avoids evaluation of the second argu-
ment, and hence takes one less reduction step.

Exercise 3

mult 3 4
= { applying mult }

(λx → (λy → x ∗ y)) 3 4
= { applying λx → (λy → x ∗ y) }

(λy → 3 ∗ y) 4
= { applying λy → 3 ∗ y }

3 ∗ 4
= { applying ∗ }

12
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Exercise 4

fibs = 0 : 1 : [x + y | (x , y)← zip fibs (tail fibs)]

Exercise 5

(1)

fib n = fibs !! n

(2)

head (dropWhile (≤ 1000) fibs)

Exercise 6

repeatTree :: a → Tree a
repeatTree x = Node t x t

where t = repeatTree x

takeTree :: Int → Tree a → Tree a
takeTree 0 = Leaf
takeTree (n + 1) Leaf = Leaf
takeTree (n + 1) (Node l x r) = Node (takeTree n l) x (takeTree n r)

replicateTree :: Int → a → Tree a
replicateTree n = takeTree n ◦ repeatTree

25



Chapter 13 - Reasoning about programs

Exercise 1

last :: [a ]→ a
last [x ] = x
last ( : xs) = last xs

or

init :: [a ]→ [a ]
init [ ] = [ ]
init (x : xs) = x : init xs

or

foldr1 :: (a → a → a)→ [a ]→ a
foldr1 [x ] = x
foldr1 f (x : xs) = f x (foldr1 f xs)

There are a number of other answers too.

Exercise 2

Base case:

add Zero (Succ m)
= { applying add }

Succ m
= { unapplying add }

Succ (add Zero m)

Inductive case:

add (Succ n) (Succ m)
= { applying add }

Succ (add n (Succ m))
= { induction hypothesis }

Succ (Succ (add n m))
= { unapplying add }

Succ (add (Succ n) m)

Exercise 3

Base case:

add Zero m
= { applying add }

m
= { property of add }

add m Zero
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Inductive case:

add (Succ n) m
= { applying add }

Succ (add n m)
= { induction hypothesis }

Succ (add m n)
= { property of add }

add m (Succ n)

Exercise 4

Base case:

all (== x ) (replicate 0 x )
= { applying replicate }

all (== x ) [ ]
= { applying all }

True

Inductive case:

all (== x ) (replicate (n + 1) x )
= { applying replicate }

all (== x ) (x : replicate n x )
= { applying all }

x == x ∧ all (== x ) (replicate n x )
= { applying == }

True ∧ all (== x ) (replicate n x )
= { applying ∧ }

all (== x ) (replicate n x )
= { induction hypothesis }

True

Exercise 5.1

Base case:

[ ] ++ [ ]
= { applying ++ }

[ ]

Inductive case:

(x : xs) ++ [ ]
= { applying ++ }

x : (xs ++ [ ])
= { induction hypothesis }

x : xs
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Exercise 5.2

Base case:

[ ] ++ (ys ++ zs)
= { applying ++ }

ys ++ zs
= { unapplying ++ }

([ ] ++ ys) ++ zs

Inductive case:

(x : xs) ++ (ys ++ zs)
= { applying ++ }

x : (xs ++ (ys ++ zs))
= { induction hypothesis }

x : ((xs ++ ys) ++ zs)
= { unapplying ++ }

(x : (xs ++ ys)) ++ zs
= { unapplying ++ }

((x : xs) ++ ys) ++ zs

Exercise 6

The three auxiliary results are all general properties that may be useful in other
contexts, whereas the single auxiliary result is specific to this application.

Exercise 7

Base case:

map f (map g [ ])
= { applying the inner map }

map f [ ]
= { applying map }

[ ]
= { unapplying map }

map (f ◦ g) [ ]

Inductive case:

map f (map g (x : xs))
= { applying the inner map }

map f (g x : map g xs)
= { applying the outer map }

f (g x ) : map f (map g xs)
= { induction hypothesis }

f (g x ) : map (f ◦ g) xs
= { unapplying ◦ }

(f ◦ g) x : map (f ◦ g) xs
= { unappling map }

map (f ◦ g) (x : xs)
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Exercise 8

Base case:

take 0 xs ++ drop 0 xs
= { applying take, drop }

[ ] ++ xs
= { applying ++ }

xs

Base case:

take (n + 1) [ ] ++ drop (n + 1) [ ]
= { applying take, drop }

[ ] ++ [ ]
= { applying ++ }

[ ]

Inductive case:

take (n + 1) (x : xs) ++ drop (n + 1) (x : xs)
= { applying take, drop }

(x : take n xs) ++ (drop n xs)
= { applying ++ }

x : (take n xs ++ drop n xs)
= { induction hypothesis }

x : xs

Exercise 9

Definitions:

leaves (Leaf ) = 1
leaves (Node l r) = leaves l + leaves r

nodes (Leaf ) = 0
nodes (Node l r) = 1 + nodes l + nodes r

Property:

leaves t = nodes t + 1

Base case:

nodes (Leaf n) + 1
= { applying nodes }

0 + 1
= { applying + }

1
= { unapplying leaves }

leaves (Leaf n)

29



Inductive case:

nodes (Node l r) + 1
= { applying nodes }

1 + nodes l + nodes r + 1
= { arithmetic }

(nodes l + 1) + (nodes r + 1)
= { induction hypotheses }

leaves l + leaves r
= { unapplying leaves }

leaves (Node l r)

Exercise 10

Base case:

comp′ (Val n) c
= { applying comp′ }

comp (Val n) ++ c
= { applying comp }

[PUSH n ] ++ c
= { applying ++ }

PUSH n : c

Inductive case:

comp′ (Add x y) c
= { applying comp′ }

comp (Add x y) ++ c
= { applying comp }

(comp x ++ comp y ++ [ADD ]) ++ c
= { associativity of ++ }

comp x ++ (comp y ++ ([ADD ] ++ c))
= { applying ++ }

comp x ++ (comp y ++ (ADD : c))
= { induction hypothesis for y }

comp x ++ (comp′ y (ADD : c))
= { induction hypothesis for x }

comp′ x (comp′ y (ADD : c))

In conclusion, we obtain:

comp′ (Val n) c = PUSH n : c
comp′ (Add x y) c = comp′ x (comp′ y (ADD : c))
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